\documentclass[a4paper,12pt]{article}
\usepackage{latexsym}
\usepackage{amsmath}
\usepackage{amssymb}
\usepackage{graphicx}
\usepackage{wrapfig}
\pagestyle{plain}
\usepackage{fancybox}
\usepackage{bm}

\begin{document}

Proof. See Appendix . Theorem 5: Under Assumptions 1-3, 5, 7-8,

a) and Assumptions $4\mathrm{a}, 6\mathrm{a}$, the total average treatment effect on compliers is

identified:
$$
\Delta_{1}^{c}=\frac{p_{1|1}}{p_{1|1}-p_{1|0}}E[Y_{1}|D=1,\ M=1]-\frac{p_{1|0}}{p_{1|1}-p_{1|0}}E[Q_{11}(Y_{0})|D=0,\ M=1]
$$
$$
-\frac{p_{0|0}}{p_{1|1}-p_{1|0}}E[Y_{1}|D=0,\ M=0]+\frac{p_{0|1}}{p_{1|1}-p_{1|0}}E[Q_{00}(Y_{0})|D=1,\ M=0].
$$
Furthermore, the total quantile treatment effect on compliers $\Delta_{1}^{c}(q)=F_{Y_{1}(1,1)|c}^{-1}(q)-$

$F_{Y_{1}(0,0)|c}^{-1}(q)$ is identified using the inverse of $()$ and $()$ .

b) and Assumptions $4\mathrm{a}, 6\mathrm{b}$, the average indirect effect under $d=0$ on compliers

is identified:

d1{\it c}(0) $=\displaystyle \frac{p_{1|1}}{p_{1|1}-p_{1|0}}E[Q_{11}(Y_{0})|D=1,\ M=1]-\frac{p_{1|0}}{p_{1|1}-p_{1|0}}E[Y_{1}|D=0,\ M=1]$
$$
-\frac{p_{0|0}}{p_{1|1}-p_{1|0}}E[Y_{1}|D=0,\ M=0]+\frac{p_{0|1}}{p_{1|1}-p_{1|0}}E[Q_{00}(Y_{0})|D=1,\ M=0].
$$
Furthermore, the quantile indirect effect under $d=0$ on compliers d1 $(q,\ 0) =$

$F_{Y_{1}(0,1)|c}^{-1}(q)-F_{Y_{1}(0,0)|c}^{-1}(q)$ is identified using the inverse of $()$ and $()$ .

c) and Assumptions $4\mathrm{b}, 6\mathrm{a}$, the average indirect effect under $d=1$ on compliers

is identified:
\begin{center}
d1 (1) $=\displaystyle \frac{p_{1|1}}{p_{1|1}-p_{1|0}}E[Y_{1}|D=1,\ M=1]-\frac{p_{1|0}}{p_{1|1}-p_{1|0}}E[Q_{11}(Y_{0})|D=0,\ M=1]$
$$
-\frac{p_{0|0}}{p_{1|1}-p_{1|0}}E[Q_{00}(Y_{0})|D=0,\ M=0]+\frac{p_{0|1}}{p_{1|1}-p_{1|0}}E[Y_{1}|D=1,\ M=0].
$$
\end{center}
Furthermore, the quantile indirect effect under $d= 1$ on compliers d1 $(q,\ 1) =$

$F_{Y_{1}(1,1)|c}^{-1}(q)-F_{Y_{1}(1,0)|c}^{-1}(q)$ is identified using the inverse of $()$ and $()$ .

Proof. See Appendix .
\end{document}
