\documentclass[a4paper,12pt]{article}
\usepackage{latexsym}
\usepackage{amsmath}
\usepackage{amssymb}
\usepackage{graphicx}
\usepackage{wrapfig}
\pagestyle{plain}
\usepackage{fancybox}
\usepackage{bm}

\begin{document}

0.1 Quantile direct effect under $\mathrm{d}=1$ conditional on $\mathrm{D}=1$

and $\mathrm{M}(1)=0$

In the following, we prove that
\begin{center}
?11,0 $(q,\ 1) = F_{Y_{1}(1,0)|D=1,M(1)=0}^{-1}(q) - F_{Y_{1}(0,0)|D=1,M(1)=0}^{-1}(q)$ ,
$$
=\ F_{Y_{1}|D=1,M=0}^{-1}(q)\ -\ F_{Q_{00}}^{-1}(Y_{0})|D=1,M=0(q)
$$
\end{center}
For this purpose, we have to show that
\begin{center}
$F_{Y_{1}(1,0)|D=1,M(1)=0}(y)=F_{Y_{1}|D=1,M=0}(y)$ and   (1)

$F_{Y_{1}(0,0)|D=1,M(1)=0}(y)=F_{Q_{00}(Y_{0})|D=1,M=0}(y)$ ,   (2)
\end{center}
which is sufficient to show that the quantiles are also identified. We can show $()$ using

the observational rule $F_{Y_{1}(1,0)|D=1,M(1)=0}(y) = F_{Y_{1}|D=1,M=0}(y) = E[1\{Y_{1}\ \leq\ y\}|D =$

$1, M=0]$, with $1\{\cdot\}$ being the indicator function. Using $()$ , we obtain
$$
F_{Q_{00}(Y_{0})|D=1,M=0}(y)
$$
$$
=E[1\{Q_{00}(Y_{0})\leq y\}|D=1,\ M=0],
$$
\begin{center}
$=E[1\{F_{Y_{1}|D=0,M=0}^{-1}\ \ovalbox{\tt\small REJECT}\ F_{Y_{0}|D=0,M=0}(Y_{0})\leq y\}|D=1,\ M=0]$,   (3)
$$
=E[1\{Y_{1}(0,0)\leq y\}|D=1,\ M=0],
$$
$$
=F_{Y_{1}(0,0)|D=1,M(1)=0}(y)\ ,
$$
\end{center}
which proves $()$ .

0.2 Average direct effect under $\mathrm{d}=0$ conditional on $\mathrm{D}=0$

and $\mathrm{M}(0)=0$

In the following, we show that ?01 $0(0) = E[Y_{1}(1,0) -Y_{1}(0,0)|D = 0, M(0) =$

$0] = E[Q_{10}(Y_{0})\ -Y_{1}|D\ =\ 0,\ M\ =\ 0]$. Using the observational rule, we obtain

$E[Y_{1}(0,0)|D=0,\ M(0)=0]=E[Y_{1}|D=0,\ M=0]$. Accordingly, we have to show
\end{document}
