\documentclass[a4paper,12pt]{article}
\usepackage{latexsym}
\usepackage{amsmath}
\usepackage{amssymb}
\usepackage{graphicx}
\usepackage{wrapfig}
\pagestyle{plain}
\usepackage{fancybox}
\usepackage{bm}

\begin{document}

0.1 Quantile direct effect under $\mathrm{d}=0$ conditional on $\mathrm{D}=0$

and $\mathrm{M}(0)=0$

In the following, we prove that
\begin{center}
?01'0 $(q,\ 0) = F_{Y_{1}(1,0)|D=0,M(0)=0}^{-1}(q) - F_{Y_{1}(0,0)|D=0,M(0)=0}^{-1}(q)$ ,
$$
=\ F_{Q_{10}}^{-1}(Y_{0})|D=0,M=0(q)\ -\ F_{Y_{1}|D=0,M=0}^{-1}(q)
$$
\end{center}
For this purpose, we have to show that
\begin{center}
$F_{Y_{1}(1,0)|D=0,M(0)=0}(y)=F_{Q_{10}(Y_{0})|D=0,M=0}(y)$ and   (1)

$F_{Y_{1}(0,0)|D=0,M(0)=0}(y)=F_{Y_{1}|D=0,M=0}(y)$ ,   (2)
\end{center}
which is sufficient to show that the quantiles are also identified. We can show $()$ using

the observational rule $F_{Y_{1}(0,0)|D=0,M(0)=0}(y) = F_{Y_{1}|D=0,M=0}(y) = E[1\{Y_{1}\ \leq\ y\}|D =$

$0, M=0]$. Using $()$ , we obtain
$$
F_{Q_{10}(Y_{0})|D=0,M=0}(y)
$$
$$
=E[1\{Q_{10}(Y_{0})\leq y\}|D=0,\ M=0],
$$
$$
=E[1\{F_{Y_{1}|D=1,M=0}^{-1}\ \ovalbox{\tt\small REJECT}\ F_{Y_{0}|D=1,M=0}(Y_{0})\leq y\}|D=0,\ M=0],
$$
$$
=E[1\{Y_{1}(1,0)\leq y\}|D=0,\ M=0],
$$
$$
=F_{Y_{1}(1,0)|D=0,M(0)=0}(y)\ ,
$$
which proves $()$ .
\end{document}
