\documentclass[a4paper,12pt]{article}
\usepackage{latexsym}
\usepackage{amsmath}
\usepackage{amssymb}
\usepackage{graphicx}
\usepackage{wrapfig}
\pagestyle{plain}
\usepackage{fancybox}
\usepackage{bm}

\begin{document}

1 Proof of Theorem 2

1.1 Average direct effect under $\mathrm{d}=0$ conditional on $\mathrm{D}=0$

and $\mathrm{M}(0)=1$

In the following, we show that ?011 (0) $= E[Y_{1}(1,1) -Y_{1}(0,1)|D = 0, M(0) =$

$1] = E[Q_{11}(Y_{0})\ -Y_{1}|D\ =\ 0,\ M\ =\ 1]$. Using the observational rule, we obtain

$E[Y_{1}(0,1)|D\ =\ 0,\ M(0)\ =\ 1] = E[Y_{1}|D\ =\ 0,\ M\ =\ 1]$. Accordingly, we have to

show that $E[Y_{1}(1,1)|D\ =\ 0,\ M(0)\ =\ 1] = E[Q_{11}(Y_{0})|D\ =\ 0,\ M\ =\ 1]$ to finish the

proof. Under Assumptions 1and $5\mathrm{a}$, the conditional potential outcome distribution

function equals
$$
F_{Y_{\mathrm{t}}(d,0)|D=1,M=0}(y)^{A1}=\mathrm{P}\mathrm{r}(h(d,\ m,\ t,\ U)\leq y|D=0,\ M=1,\ T=t)\ ,
$$
$$
=\mathrm{P}\mathrm{r}(U\leq h^{-1}(d,\ m,\ t;y)|D=0,\ M=1,\ T=t)\ ,
$$
(1)
$$
A5a=\mathrm{P}\mathrm{r}(U\leq h^{-1}(d,\ m,\ t;y)|D=0,\ M=1)\ ,
$$
$$
=F_{U|01}(h^{-1}(d,\ m,\ t;y))\ ,
$$
for $d, d' \in \{0$, 1$\}$. We use these quantities in the following. First, evaluating

$F_{Y_{1}(1,1)|D=0,M=1}(y)$ at $h(1,1,1,\ u)$ gives
$$
F_{Y_{1}(1,1)|D=0,M=1}(h(1,1,1,\ u))=F_{U|01}(h^{-1}(1,1,1;h(1,1,1,\ u)))=F_{U|01}(u)\ .
$$
Applying $F_{Y_{1}(1,1)|D=0,M=1}^{-1}(q)$ to both sides, we have
\begin{center}
$h(1,1,1,\ u)=F_{Y_{1}(1,1)|D=0,M=1}^{-1}(F_{U|01}(u))$ .   (2)
\end{center}
Second, for $F_{Y_{0}(1,1)|D=0,M=1}(y)$ we have
\begin{center}
$F_{U|01}^{-1}(F_{Y_{0}(1,1)|D=0,M=1}(y))=h^{-1}(1,1,0;y)$ .   (3)
\end{center}\end{document}
