\documentclass[a4paper,12pt]{article}
\usepackage{latexsym}
\usepackage{amsmath}
\usepackage{amssymb}
\usepackage{graphicx}
\usepackage{wrapfig}
\pagestyle{plain}
\usepackage{fancybox}
\usepackage{bm}

\begin{document}

1 Proof of Theorem 3

1.1 Average direct effect on the never-takers

In the following, we show that $ё n1=E[Y_{1}(1,0)-Y_{1}(0,\ 0)|Д\ =n]=E[Y_{1}-Q_{00}(Y_{0})|D=$

$1, M = 0]$. From $()$ , we obtain the first ingredient $E[Y_{1}(1,\ 0)|Д\ =\ n] = E[Y_{1}|D =$

$1, M=0]$. Furthermore, from $()$ we have $E[Q_{00}(Y_{0})|D=1,\ M=0]=E[Y_{1}(0,0)|D=$

$1, M(1)=0]$. Under Assumption7and 8,
$$
E[Y_{1}(0,0)|D=1,\ M(1)=0]^{A7}=E[Y_{1}(0,0)|D=1,\ Д\ =n]
$$
(1)
$$
A8=E[Y_{1}\ (0,\ 0)|Д\ =n].
$$
1.2 Quantile direct effect on the never-takers

We prove that
\begin{center}
?$n$1 ($q$) $= F_{Y_{1}(1,0)|Д=n}^{-1}(q) - F_{Y_{1}(0,0)|Д=n}^{-1}(q)$ ,
$$
=\ F_{Y_{1}|D=1,M=0}^{-1}(q)\ -\ F_{Q_{00}(Y_{0})|D=1,M=0}^{-1}(q)
$$
\end{center}
This requires showing that
\begin{center}
$F_{Y_{1}(1,0)|Д=n}(y)=F_{Y_{1}|D=1,M=0}(y)$ and   (2)

$F_{Y_{1}}$ (0,0)$|$t $=n(y) = F_{Q_{00}(Y_{0})|D=1,M=0}(y)$   (3)
\end{center}
Under Assumptions 7 and 8,
$$
F_{Y_{\mathrm{t}}|D=1,M=0}(y)=E[1\{Y_{t}\leq y\}|D=1,\ M=0]
$$
\begin{center}
$A7,A8=E[1\{Y_{t}(1,0)\ \leq\ y\}|Д\ =n]$   (4)

$= F_{Y_{\mathrm{t}}}$ (1,0)$|$t $=n(y)$ ,
\end{center}
which proves $()$ . From $()$ , we have

$F_{Q_{00}(Y_{0})|D=1,M=0}(y)=F_{Y_{1}(0,0)|D=1,M(1)=0}(y)=E[1\{Y_{1}(0,0)\ \leq y\}|D=1,\ M(1)=0].$
\end{document}
