\documentclass[a4paper,12pt]{article}
\usepackage{latexsym}
\usepackage{amsmath}
\usepackage{amssymb}
\usepackage{graphicx}
\usepackage{wrapfig}
\pagestyle{plain}
\usepackage{fancybox}
\usepackage{bm}

\begin{document}

Under Assumption 7 and 8,
$$
E[1\{Y_{1}(0,0)\leq y\}|D=1,\ M(1)=0]^{A7}=^{A8}E[1\{Y_{1}(0,0)\ \leq\ y\}|Д\ =n]
$$
(1)
$$
=F_{Y_{1}(0,0)|Д=n}(y)\ ,
$$
which proves.

0.1 Average direct effect under $\mathrm{d}=0$ on compliers

In the following, we show that
\begin{center}
?1 (0) $=E[Y_{1}(1,0)-Y_{1}(0,\ 0)|Д\ =c],$
$$
=\frac{p_{0|0}}{p_{0|0}-p_{0|1}}E[Q_{10}(Y_{0})-Y_{1}|D=0,\ M=0]
$$
$$
-\frac{p_{0|1}}{p_{0|0}-p_{0|1}}E[Y_{1}-Q_{00}(Y_{0})|D=1,\ M=0].
$$
\end{center}
Plugging $()$ in $()$ under $T=1$, we obtain
$$
E[Y_{1}|D=0,\ M=0]=\frac{p_{n}}{p_{n}+p_{c}}E[Q_{00}(Y_{0})|D=1,\ M=0]
$$
$$
+\frac{p_{c}}{p_{n}+p_{c}}E[Y_{1}\ (0,\ 0)|Д\ =c].
$$
This allows identifying
$$
E[Y_{1}\ (0,\ 0)|Д\ =c]\ =\frac{p_{0|0}}{p_{0|0}-p_{0|1}}E[Y_{1}|D=0,\ M=0]
$$
(2)
$$
-\frac{p_{0|1}}{p_{0|0}-p_{0|1}}E[Q_{00}(Y_{0})|D=1,\ M=0].
$$
Accordingly, we have to show the identification of $E[Y_{1}(1,0)|c]$ to finish the proof.

From $()$ we have $E[Y_{1}(1,0)|D=0,\ M=0]=E[Q_{10}(Y_{0})|D=0,\ M=0]$. Applying
\end{document}
