\documentclass[a4paper,12pt]{article}
\usepackage{latexsym}
\usepackage{amsmath}
\usepackage{amssymb}
\usepackage{graphicx}
\usepackage{wrapfig}
\pagestyle{plain}
\usepackage{fancybox}
\usepackage{bm}

\begin{document}

0.1 Average direct effect under $\mathrm{d}=1$ on compliers

In the following, we show that
\begin{center}
?1 (1) $=E[Y_{1}(1,1)-Y_{1}(0,\ 1)|Д\ =c],$
$$
=\frac{p_{1|1}}{p_{1|1}-p_{1|0}}E[Y_{1-}Q01(Y_{0})|D=1,\ M=1]
$$
$$
-\frac{p_{1|0}}{p_{1|1}-p_{1|0}}E[Q_{11}(Y_{0})-Y_{1}|D=0,\ M=1].
$$
\end{center}
Plugging $()$ in $()$ , we obtain
$$
E[Y_{1}|D=1,\ M=1]\ =\frac{p_{a}}{p_{a}+p_{c}}E[Q_{11}(Y_{0})|D=0,\ M=1]
$$
$$
+\frac{p_{c}}{p_{a}+p_{c}}E[Y_{1}\ (1,\ 1)|Д=c].
$$
This allows identifying
$$
E[Y_{1}\ (1,\ 1)|Д=c]=\frac{p_{1|1}}{p_{1|1}-p_{1|0}}E[Y_{1}|D=1,\ M=1]
$$
(1)
$$
-\frac{p_{1|0}}{p_{1|1}-p_{1|0}}E[Q_{11}(Y_{0})|D=0,\ M=1].
$$
From $()$ we have $E[Y_{1}(0,1)|D=\ 1,\ M=\ 1] =E[Q_{01}(Y_{0})|D=\ 1,\ M=\ 1]$. Applying

the law of iterative expectations, gives
$$
E[Y_{1}(0,1)|D=1,\ M=1]=\frac{p_{a}}{p_{a}+p_{c}}E[Y_{1}(0,1)|D=1,\ M=1,\ Д\ =a]
$$
$$
+\frac{p_{c}}{p_{a}+p_{c}}E[Y_{1}(0,1)|D=1,\ M=1,\ Д\ =c],
$$
$$
A7=\frac{p_{a}}{p_{a}+p_{c}}E[Y_{1}\ (0,\ 1)|Д\ =a]+\frac{p_{c}}{p_{a}+p_{c}}E[Y_{1}(0,\ 1)|Д\ =c].
$$
After some rearrangements and using $()$ , we obtain

$E[Y_{1}\ (0,\ 1)|Д\ =c] =\displaystyle \frac{p_{a}+p_{c}}{p_{c}}E[Q_{01}(Y_{0})|D=1,\ M=1]-\frac{p_{a}}{p_{c}}E[Y_{1}|D=0,\ M=1].$
\end{document}
