\documentclass[a4paper,12pt]{article}
\usepackage{latexsym}
\usepackage{amsmath}
\usepackage{amssymb}
\usepackage{graphicx}
\usepackage{wrapfig}
\pagestyle{plain}
\usepackage{fancybox}
\usepackage{bm}

\begin{document}

Using $()$ and rearranging the equation gives

$F_{Y_{1}(1,1)|Д=c}(y)=\displaystyle \frac{p_{1|1}}{p_{1|1}-p_{1|0}}F_{Y_{1}|D=1,M=1}(y)-\frac{p_{1|0}}{p_{1|1}-p_{1|0}}F_{Q_{11}(Y_{0})|D=0,M=1}(y)$ . (1)

From $()$ , we have $F_{Y_{1}(0,1)|D=1,M(1)=1}(y) = F_{Q_{01}(Y_{0})|D=1,M=1}(y)$ . Applying the law of

iterative expectations gives
$$
F_{Y_{1}}(0,1)|D=1,M(1)=1(y)\ =\ \frac{p_{a}}{p_{a}+p_{c}}F_{Y_{1}}(0,1)|D=1,M(1)=1,Д=a(y)
$$
$$
+\frac{p_{c}}{p_{a}+p_{c}}F_{Y_{1}}(0,1)|D=1,M(1)=1,Д=c(y)\ ,
$$
\begin{center}
$A7= \displaystyle \frac{p_{a}}{p_{a}+p_{c}}F_{Y_{1}}$ (0,1)$|$t $=a(y) + \displaystyle \frac{p_{c}}{p_{a}+p_{c}}F_{Y_{1}}$ (0,1)$|$t $=c(y)$
\end{center}
Using $()$ and rearranging the equation gives,

$F_{Y_{1}(0,1)|Д=c}(y)=\displaystyle \frac{p_{1|1}}{p_{1|1}-p_{1|0}}F_{Q_{01}(Y_{0})|D=1,M=1}(y)-\frac{p_{1|0}}{p_{1|1}-p_{1|0}}F_{Y_{1}|D=0,M=1}(y)$ . (2)

1 Proof of Theorem 5

1.1 Average treatment effect on the compliers

In $()$ and $()$ , we show that
$$
ё 1=E[Y_{1}(1,1)-Y_{1}(0,\ 0)|Д\ =c],
$$
$$
=\frac{p_{1|1}}{p_{1|1}-p_{1|0}}E[Y_{1}|D=1,\ M=1]-\frac{p_{1|0}}{p_{1|1}-p_{1|0}}E[Q_{11}(Y_{0})|D=0,\ M=1]
$$
$$
-\frac{p_{0|0}}{p_{0|0}-p_{0|1}}E[Y_{1}|D=0,\ M=0]+\frac{p_{0|1}}{p_{0|0}-p_{0|1}}E[Q_{00}(Y_{0})|D=1,\ M=0].
$$
1.2 Quantile treatment effect on the compliers

In $()$ and $()$ , we show that $F_{Y_{1}(1,1)|c}(y)$ and $F_{Y_{1}(0,0)|c}(y)$ are identified. Accordingly,

$\Delta_{1}^{c}(q)=F^{-1}Y_{1}(1,1)|c(q)-F_{Y_{1}(0,0)|c}^{-1}(q)$ is identified.
\end{document}
