\documentclass[a4paper,12pt]{article}
\usepackage{latexsym}
\usepackage{amsmath}
\usepackage{amssymb}
\usepackage{graphicx}
\usepackage{wrapfig}
\pagestyle{plain}
\usepackage{fancybox}
\usepackage{bm}

\begin{document}

0.1 Average indirect effect under $d=0$ on compliers

In $()$ and $()$ , we show that
\begin{center}
d1 (0) $=E[Y_{1}(0,1)-Y_{1}(0,\ 0)|Д\ =c],$
$$
=\frac{p_{1|1}}{p_{1|1}-p_{1|0}}E[Q_{11}(Y_{0})|D=1,\ M=1]-\frac{p_{1|0}}{p_{1|1}-p_{1|0}}E[Y_{1}|D=0,\ M=1]
$$
$$
-\frac{p_{0|0}}{p_{0|0}-p_{0|1}}E[Y_{1}|D=0,\ M=0]+\frac{p_{0|1}}{p_{0|0}-p_{0|1}}E[Q_{00}(Y_{0})|D=1,\ M=0].
$$
\end{center}
0.2 Quantile indirect effect under $d=0$ on compliers

In $()$ and $()$ , we show that $F_{Y_{1}(0,1)|c}(y)$ and $F_{Y_{1}(0,0)|c}(y)$ are identified. Accordingly,

d1{\it c} $(q,\ 0) = F^{-1}Y_{1}(0,1)|c(q)$ -- $F_{Y_{1}(0,0)|c}^{-1}(q)$ is identified.

0.3 Average indirect effect under $d=1$ on compliers

In $()$ and $()$ , we show that
\begin{center}
d1 (1) $=E[Y_{1}(1,1)-Y_{1}(1,\ 0)|Д\ =c],$
$$
=\frac{p_{1|1}}{p_{1|1}-p_{1|0}}E[Y_{1}|D=1,\ M=1]-\frac{p_{1|0}}{p_{1|1}-p_{1|0}}E[Q_{11}(Y_{0})|D=0,\ M=1]
$$
$$
-\frac{p_{0|0}}{p_{0|0}-p_{0|1}}E[Q_{00}(Y_{0})|D=0,\ M=0]+\frac{p_{0|1}}{p_{0|0}-p_{0|1}}E[Y_{1}|D=1,\ M=0].
$$
\end{center}
0.4 Quantile indirect effect under $d=1$ on compliers

In $()$ and $()$ , we show that $F_{Y_{1}(1,1)|c}(y)$ and $F_{Y_{1}(1,0)|c}(y)$ are identified. Accordingly,

d1{\it c} $(q,\ 1)=F^{-1}Y_{1}(1,1)|c(q)-F_{Y_{1}(1,0)|c}^{-1}(q)$ is identified.
\end{document}
